\documentclass[12pt]{article}
\usepackage{amsmath}
\usepackage{amssymb}
\usepackage{geometry}
\geometry{a4paper, margin=0.5in}

\begin{document}

\section*{Question 1}
Solve the given linear system by any method.

\subsection*{(i)}
\begin{align*}
2x_1 + x_2 + 3x_3 &= 0\\
x_1 + 2x_2 &= 0\\
x_2 + x_3 &= 0
\end{align*}

\textbf{Solution using Reduced Row Echelon Form:}

Setting up the augmented matrix:
\[
\left(\begin{array}{ccc|c}
2 & 1 & 3 & 0\\
1 & 2 & 0 & 0\\
0 & 1 & 1 & 0
\end{array}\right)
\]

Step 1: $R_1 \leftrightarrow R_2$ (swap rows to get leading 1)
\[
\left(\begin{array}{ccc|c}
1 & 2 & 0 & 0\\
2 & 1 & 3 & 0\\
0 & 1 & 1 & 0
\end{array}\right)
\]

Step 2: $R_2 \leftarrow R_2 - 2R_1$ (eliminate below pivot)
\[
\left(\begin{array}{ccc|c}
1 & 2 & 0 & 0\\
0 & -3 & 3 & 0\\
0 & 1 & 1 & 0
\end{array}\right)
\]

Step 3: $R_2 \leftarrow -\frac{1}{3}R_2$ (make leading coefficient 1)
\[
\left(\begin{array}{ccc|c}
1 & 2 & 0 & 0\\
0 & 1 & -1 & 0\\
0 & 1 & 1 & 0
\end{array}\right)
\]

Step 4: $R_3 \leftarrow R_3 - R_2$ (eliminate below pivot)
\[
\left(\begin{array}{ccc|c}
1 & 2 & 0 & 0\\
0 & 1 & -1 & 0\\
0 & 0 & 2 & 0
\end{array}\right)
\]

Step 5: $R_3 \leftarrow \frac{1}{2}R_3$ (make leading coefficient 1)
\[
\left(\begin{array}{ccc|c}
1 & 2 & 0 & 0\\
0 & 1 & -1 & 0\\
0 & 0 & 1 & 0
\end{array}\right)
\]

Step 6: $R_2 \leftarrow R_2 + R_3$ (eliminate above pivot in column 3)
\[
\left(\begin{array}{ccc|c}
1 & 2 & 0 & 0\\
0 & 1 & 0 & 0\\
0 & 0 & 1 & 0
\end{array}\right)
\]

Step 7: $R_1 \leftarrow R_1 - 2R_2$ (eliminate above pivot in column 2)
\[
\left(\begin{array}{ccc|c}
1 & 0 & 0 & 0\\
0 & 1 & 0 & 0\\
0 & 0 & 1 & 0
\end{array}\right)
\]

From the reduced row echelon form, we get:
\begin{align*}
x_1 &= 0\\
x_2 &= 0\\
x_3 &= 0
\end{align*}

Therefore, the solution is $\boxed{(x_1, x_2, x_3) = (0, 0, 0)}$.

\subsection*{(ii)}
\begin{align*}
2x - y - 3z &= 0\\
-x + 2y - 3z &= 0\\
x + y + 4z &= 0
\end{align*}

\textbf{Solution using Elimination Method:}

Given system:
\begin{align}
2x - y - 3z &= 0 \quad (1)\\
-x + 2y - 3z &= 0 \quad (2)\\
x + y + 4z &= 0 \quad (3)
\end{align}

Step 1: Eliminate $x$ from equations (1) and (2)
Multiply equation (2) by 2: $-2x + 4y - 6z = 0$
Add to equation (1): $(2x - y - 3z) + (-2x + 4y - 6z) = 0$
\begin{align}
3y - 9z &= 0 \quad (4)
\end{align}

Step 2: Eliminate $x$ from equations (2) and (3)
Add equations (2) and (3): $(-x + 2y - 3z) + (x + y + 4z) = 0$
\begin{align}
3y + z &= 0 \quad (5)
\end{align}

Step 3: Solve the system of equations (4) and (5)
From equation (4): $3y - 9z = 0 \Rightarrow y = 3z$
Substitute into equation (5): $3(3z) + z = 0$
\begin{align*}
9z + z &= 0\\
10z &= 0\\
z &= 0
\end{align*}

Step 4: Find $y$ and $x$
Since $z = 0$ and $y = 3z$:
\begin{align*}
y &= 3(0) = 0
\end{align*}

Substitute $y = 0$ and $z = 0$ into equation (3):
\begin{align*}
x + 0 + 4(0) &= 0\\
x &= 0
\end{align*}

Verification: Let's check our solution $(x, y, z) = (0, 0, 0)$ in all three original equations:
\begin{align*}
\text{Equation (1):} \quad 2(0) - 0 - 3(0) &= 0 \quad \checkmark\\
\text{Equation (2):} \quad -0 + 2(0) - 3(0) &= 0 \quad \checkmark\\
\text{Equation (3):} \quad 0 + 0 + 4(0) &= 0 \quad \checkmark
\end{align*}

Therefore, the solution is $\boxed{(x, y, z) = (0, 0, 0)}$.

\subsection*{(iii)}
\begin{align*}
v + 3w - 2x &= 0\\
2u + v - 4w + 3x &= 0\\
2u + 3v + 2w - x &= 0\\
-4u - 3v + 5w - 4x &= 0
\end{align*}

\textbf{Solution using Row Echelon Form:}

Reordering variables as $u, v, w, x$ and setting up the augmented matrix:
\[
\left(\begin{array}{cccc|c}
0 & 1 & 3 & -2 & 0\\
2 & 1 & -4 & 3 & 0\\
2 & 3 & 2 & -1 & 0\\
-4 & -3 & 5 & -4 & 0
\end{array}\right)
\]

Step 1: $R_1 \leftrightarrow R_2$ (get non-zero leading element)
\[
\left(\begin{array}{cccc|c}
2 & 1 & -4 & 3 & 0\\
0 & 1 & 3 & -2 & 0\\
2 & 3 & 2 & -1 & 0\\
-4 & -3 & 5 & -4 & 0
\end{array}\right)
\]

Step 2: $R_1 \leftarrow \frac{1}{2}R_1$ (make leading coefficient 1)
\[
\left(\begin{array}{cccc|c}
1 & \frac{1}{2} & -2 & \frac{3}{2} & 0\\
0 & 1 & 3 & -2 & 0\\
2 & 3 & 2 & -1 & 0\\
-4 & -3 & 5 & -4 & 0
\end{array}\right)
\]

Step 3: $R_3 \leftarrow R_3 - 2R_1$ and $R_4 \leftarrow R_4 + 4R_1$
\[
\left(\begin{array}{cccc|c}
1 & \frac{1}{2} & -2 & \frac{3}{2} & 0\\
0 & 1 & 3 & -2 & 0\\
0 & 2 & 6 & -4 & 0\\
0 & -1 & -3 & 2 & 0
\end{array}\right)
\]

Step 4: $R_3 \leftarrow R_3 - 2R_2$ and $R_4 \leftarrow R_4 + R_2$
\[
\left(\begin{array}{cccc|c}
1 & \frac{1}{2} & -2 & \frac{3}{2} & 0\\
0 & 1 & 3 & -2 & 0\\
0 & 0 & 0 & 0 & 0\\
0 & 0 & 0 & 0 & 0
\end{array}\right)
\]

The system reduces to:
\begin{align*}
u + \frac{1}{2}v - 2w + \frac{3}{2}x &= 0\\
v + 3w - 2x &= 0
\end{align*}

\textbf{Solution using Equation Elimination:}

Given system:
\begin{align}
v + 3w - 2x &= 0 \quad (1)\\
2u + v - 4w + 3x &= 0 \quad (2)\\
2u + 3v + 2w - x &= 0 \quad (3)\\
-4u - 3v + 5w - 4x &= 0 \quad (4)
\end{align}

Step 1: Eliminate $u$ from equations (2) and (3)
Subtract equation (2) from (3): $(2u + 3v + 2w - x) - (2u + v - 4w + 3x) = 0$
\begin{align}
2v + 6w - 4x &= 0 \quad (5)
\end{align}

Step 2: Eliminate $u$ from equations (2) and (4)
Multiply equation (2) by 2: $4u + 2v - 8w + 6x = 0$
Add to equation (4): $(4u + 2v - 8w + 6x) + (-4u - 3v + 5w - 4x) = 0$
\begin{align}
-v - 3w + 2x &= 0 \quad (6)
\end{align}

Step 3: Compare equations (1) and (6)
From equation (1): $v + 3w - 2x = 0$
From equation (6): $-v - 3w + 2x = 0$

Adding these equations: $(v + 3w - 2x) + (-v - 3w + 2x) = 0$
This gives us: $0 = 0$ (always true)

This means equations (1) and (6) are equivalent, confirming our system has infinite solutions.

\textbf{General Solution:}

From the reduced system, we can express $u$ and $v$ in terms of free variables $w$ and $x$:

From equation (1): $v = 2x - 3w$

Substituting into the first reduced equation:
$u + \frac{1}{2}(2x - 3w) - 2w + \frac{3}{2}x = 0$
$u + x - \frac{3w}{2} - 2w + \frac{3x}{2} = 0$
$u = -\frac{5x}{2} + \frac{7w}{2}$

Therefore, the general solution is:
\begin{align*}
u &= \frac{7w - 5x}{2}\\
v &= 2x - 3w\\
w &= w \quad \text{(free parameter)}\\
x &= x \quad \text{(free parameter)}
\end{align*}

Or in parametric form with parameters $s = w$ and $t = x$:
\[
\boxed{(u, v, w, x) = \left(\frac{7s - 5t}{2}, 2t - 3s, s, t\right)}
\]
where $s, t \in \mathbb{R}$ are arbitrary parameters.

\section*{Question 2}
Solve the system by Gaussian elimination.

\subsection*{(i)}
\begin{align*}
x_1 + x_2 + 2x_3 &= 8\\
-x_1 - 2x_2 + 3x_3 &= 1\\
3x_1 - 7x_2 + 4x_3 &= 10
\end{align*}

\subsection*{(ii)}
\begin{align*}
2x_1 + 2x_2 + 2x_3 &= 0\\
-2x_1 + 5x_2 + 2x_3 &= 1\\
8x_1 + x_2 + 4x_3 &= -1
\end{align*}

\section*{Question 3}
Find the inverse of Matrix.

\subsection*{(i)}
\[
\begin{pmatrix}
\frac{1}{2}(e^x + e^{-x}) & \frac{1}{2}(e^x - e^{-x})\\
\frac{1}{2}(e^x - e^{-x}) & \frac{1}{2}(e^x + e^{-x})
\end{pmatrix}
\]

\subsection*{(ii)}
\[
\begin{pmatrix}
\cos\theta & \sin\theta\\
-\sin\theta & \cos\theta
\end{pmatrix}
\]

\subsection*{(iii)}
\[
\begin{pmatrix}
1 & 2 & 3\\
2 & 5 & 3\\
1 & 0 & 8
\end{pmatrix}
\]

\subsection*{(iv)}
\[
\begin{pmatrix}
-1 & 3 & -4\\
2 & 4 & 1\\
-4 & 2 & -9
\end{pmatrix}
\]

\subsection*{(v)}
\[
\begin{pmatrix}
\frac{1}{5} & \frac{1}{5} & -\frac{2}{5}\\
\frac{1}{5} & \frac{1}{5} & \frac{1}{10}\\
\frac{1}{5} & -\frac{4}{5} & \frac{1}{10}
\end{pmatrix}
\]

\subsection*{(vi)}
\[
\begin{pmatrix}
\frac{1}{5} & \frac{1}{5} & -\frac{2}{5}\\
\frac{2}{5} & -\frac{3}{5} & -\frac{3}{10}\\
\frac{1}{5} & -\frac{4}{5} & \frac{1}{10}
\end{pmatrix}
\]

\section*{Question 4}
Systems with Parameters
\[
\begin{aligned}
4x_1 - 7x_2 &= b_1\\
x_1 + 2x_2 &= b_2
\end{aligned}
\]

\begin{itemize}
\item[(i)] $b_1 = 0, b_2 = 1$
\item[(ii)] $b_1 = -4, b_2 = 6$
\item[(iii)] $b_1 = -1, b_2 = 3$
\item[(iv)] $b_1 = -5, b_2 = 1$
\end{itemize}

\end{document}