\documentclass[12pt]{article}
\usepackage{amsmath}
\usepackage{amssymb}
\usepackage{geometry}
\geometry{a4paper, margin=0.5in}

\begin{document}

\section*{Question 1}
Solve the given linear system by any method.

% BEGIN QUESTION 1 PART 1
\subsection*{(i)}
\[
	2x_1 + x_2 + 3x_3 = 0 \quad (1)
\]
\[
	x_1 + 2x_2 = 0 \quad (2)
\]
\[
	x_2 + x_3 = 0 \quad (3)
\]

From equation (3): $x_3 = -x_2$

Substitute into equation (1):
\[
	2x_1 + x_2 + 3(-x_2) = 0
\]
\[
	2x_1 + x_2 - 3x_2 = 0
\]
\[
	2x_1 - 2x_2 = 0
\]
\[
	x_1 - x_2 = 0 \quad (4)
\]

Now we have:
\[
	x_1 - x_2 = 0 \quad (4)
\]
\[
	x_1 + 2x_2 = 0 \quad (2)
\]

Subtract equation (4) from equation (2):
\[
	(x_1 + 2x_2) - (x_1 - x_2) = 0 - 0
\]
\[
	x_1 + 2x_2 - x_1 + x_2 = 0
\]
\[
	3x_2 = 0
\]
\[
	x_2 = 0
\]

From equation (4): $x_1 = x_2 = 0$

From equation (3): $x_3 = -x_2 = 0$

Therefore: $x_1 = 0, x_2 = 0, x_3 = 0$
% END QUESTION 1 PART 1

% BEGIN QUESTION 1 PART 2
\subsection*{(ii)}
\[
	2x - y - 3z = 0
\]
\[
	-x + 2y - 3z = 0
\]
\[
	x + y + 4z = 0
\]

\[
	\begin{pmatrix}
		2  & -1 & -3 & 0 \\
		-1 & 2  & -3 & 0 \\
		1  & 1  & 4  & 0
	\end{pmatrix}
\]

$R_1 \times \frac{1}{2}$:
\[
	\begin{pmatrix}
		1  & -\frac{1}{2} & -\frac{3}{2} & 0 \\
		-1 & 2           & -3           & 0 \\
		1  & 1           & 4            & 0
	\end{pmatrix}
\]

$R_2 + R_1$:
\[
	\begin{pmatrix}
		1 & -\frac{1}{2} & -\frac{3}{2} & 0 \\
		0 & \frac{3}{2}  & -\frac{9}{2} & 0 \\
		1 & 1           & 4            & 0
	\end{pmatrix}
\]

$R_3 - R_1$:
\[
	\begin{pmatrix}
		1 & -\frac{1}{2} & -\frac{3}{2} & 0 \\
		0 & \frac{3}{2}  & -\frac{9}{2} & 0 \\
		0 & \frac{3}{2}  & \frac{11}{2} & 0
	\end{pmatrix}
\]

$R_2 \times \frac{2}{3}$:
\[
	\begin{pmatrix}
		1 & -\frac{1}{2} & -\frac{3}{2} & 0 \\
		0 & 1           & -3           & 0 \\
		0 & \frac{3}{2}  & \frac{11}{2} & 0
	\end{pmatrix}
\]

$R_3 - \frac{3}{2}R_2$:
\[
	\begin{pmatrix}
		1 & -\frac{1}{2} & -\frac{3}{2} & 0 \\
		0 & 1           & -3           & 0 \\
		0 & 0           & 10           & 0
	\end{pmatrix}
\]

$R_3 \times \frac{1}{10}$:
\[
	\begin{pmatrix}
		1 & -\frac{1}{2} & -\frac{3}{2} & 0 \\
		0 & 1           & -3           & 0 \\
		0 & 0           & 1            & 0
	\end{pmatrix}
\]

Back substitution:
\[
	z = 0
\]
\[
	y - 3z = 0 \Rightarrow y = 0
\]
\[
	x - \frac{1}{2}y - \frac{3}{2}z = 0 \Rightarrow x = 0
\]

Therefore: $x = 0, y = 0, z = 0$
% END QUESTION 1 PART 2

% BEGIN QUESTION 1 PART 3
\subsection*{(iii)}
\[
	v + 3w - 2x = 0
\]
\[
	2u + v - 4w + 3x = 0
\]
\[
	2u + 3v + 2w - x = 0
\]
\[
	-4u - 3v + 5w - 4x = 0
\]

\[
	\begin{pmatrix}
		0  & 1  & 3  & -2 & 0 \\
		2  & 1  & -4 & 3  & 0 \\
		2  & 3  & 2  & -1 & 0 \\
		-4 & -3 & 5  & -4 & 0
	\end{pmatrix}
\]

$Swap\ R_1\ with\ R_2$:
\[
	\begin{pmatrix}
		2  & 1  & -4 & 3  & 0 \\
		0  & 1  & 3  & -2 & 0 \\
		2  & 3  & 2  & -1 & 0 \\
		-4 & -3 & 5  & -4 & 0
	\end{pmatrix}
\]

$R_1 \times \frac{1}{2}$:
\[
	\begin{pmatrix}
		1  & \frac{1}{2} & -2 & \frac{3}{2} & 0 \\
		0  & 1           & 3  & -2          & 0 \\
		2  & 3           & 2  & -1          & 0 \\
		-4 & -3          & 5  & -4          & 0
	\end{pmatrix}
\]

$R_3 - 2R_1$:
\[
	\begin{pmatrix}
		1 & \frac{1}{2} & -2 & \frac{3}{2} & 0 \\
		0 & 1           & 3  & -2          & 0 \\
		0 & 2           & 6  & -4          & 0 \\
		-4 & -3          & 5  & -4          & 0
	\end{pmatrix}
\]

$R_4 + 4R_1$:
\[
	\begin{pmatrix}
		1 & \frac{1}{2} & -2 & \frac{3}{2} & 0 \\
		0 & 1           & 3  & -2          & 0 \\
		0 & 2           & 6  & -4          & 0 \\
		0 & -1          & -3 & 2           & 0
	\end{pmatrix}
\]

$R_3 - 2R_2$:
\[
	\begin{pmatrix}
		1 & \frac{1}{2} & -2 & \frac{3}{2} & 0 \\
		0 & 1           & 3  & -2          & 0 \\
		0 & 0           & 0  & 0           & 0 \\
		0 & -1          & -3 & 2           & 0
	\end{pmatrix}
\]

$R_4 + R_2$:
\[
	\begin{pmatrix}
		1 & \frac{1}{2} & -2 & \frac{3}{2} & 0 \\
		0 & 1           & 3  & -2          & 0 \\
		0 & 0           & 0  & 0           & 0 \\
		0 & 0           & 0  & 0           & 0
	\end{pmatrix}
\]

From the matrix:
\[
	u + \frac{1}{2}v - 2w + \frac{3}{2}x = 0
\]
\[
	v + 3w - 2x = 0
\]

This system has infinitely many solutions because last two rows of the matrix are all zeros.
% END QUESTION 1 PART 3

\section*{Question 2}
Solve the system by Gaussian elimination.

% BEGIN QUESTION 2 PART 1
\subsection*{(i)}
\[
	x_1 + x_2 + 2x_3 = 8
\]
\[
	-x_1 - 2x_2 + 3x_3 = 1
\]
\[
	3x_1 - 7x_2 + 4x_3 = 10
\]

\[
	\begin{pmatrix}
		1  & 1  & 2 & 8  \\
		-1 & -2 & 3 & 1  \\
		3  & -7 & 4 & 10
	\end{pmatrix}
\]

$R_2 + R_1$:
\[
	\begin{pmatrix}
		1 & 1   & 2  & 8   \\
		0 & -1  & 5  & 9   \\
		3  & -7 & 4 & 10
	\end{pmatrix}
\]

$R_3 - 3R_1$:
\[
	\begin{pmatrix}
		1 & 1   & 2  & 8   \\
		0 & -1  & 5  & 9   \\
		0 & -10 & -2 & -14
	\end{pmatrix}
\]

$R_2 \times (-1)$:
\[
	\begin{pmatrix}
		1 & 1   & 2  & 8   \\
		0 & 1   & -5 & -9  \\
		0 & -10 & -2 & -14
	\end{pmatrix}
\]

$R_3 + 10R_2$:
\[
	\begin{pmatrix}
		1 & 1 & 2   & 8    \\
		0 & 1 & -5  & -9   \\
		0 & 0 & -52 & -104
	\end{pmatrix}
\]

$R_3 \times (-\frac{1}{52})$:
\[
	\begin{pmatrix}
		1 & 1 & 2  & 8  \\
		0 & 1 & -5 & -9 \\
		0 & 0 & 1  & 2
	\end{pmatrix}
\]

Back substitution:
\[
	x_3 = 2
\]
\[
	x_2 - 5x_3 = -9 \Rightarrow x_2 = -9 + 5(2) = 1
\]
\[
	x_1 + x_2 + 2x_3 = 8 \Rightarrow x_1 = 8 - 1 - 2(2) = 3
\]

Therefore: $x_1 = 3, x_2 = 1, x_3 = 2$
% END QUESTION 2 PART 1

% BEGIN QUESTION 2 PART 2
\subsection*{(ii)}
\[
	2x_1 + 2x_2 + 2x_3 = 0
\]
\[
	-2x_1 + 5x_2 + 2x_3 = 1
\]
\[
	8x_1 + x_2 + 4x_3 = -1
\]

\[
	\begin{pmatrix}
		2  & 2 & 2 & 0  \\
		-2 & 5 & 2 & 1  \\
		8  & 1 & 4 & -1
	\end{pmatrix}
\]

$R_1 \times \frac{1}{2}$:
\[
	\begin{pmatrix}
		1  & 1 & 1 & 0  \\
		-2 & 5 & 2 & 1  \\
		8  & 1 & 4 & -1
	\end{pmatrix}
\]

$R_2 + 2R_1$:
\[
	\begin{pmatrix}
		1 & 1  & 1  & 0  \\
		0 & 7  & 4  & 1  \\
		8  & 1 & 4 & -1
	\end{pmatrix}
\]

$R_3 - 8R_1$:
\[
	\begin{pmatrix}
		1 & 1  & 1  & 0  \\
		0 & 7  & 4  & 1  \\
		0 & -7 & -4 & -1
	\end{pmatrix}
\]

$R_3 + R_2$:
\[
	\begin{pmatrix}
		1 & 1 & 1 & 0 \\
		0 & 7 & 4 & 1 \\
		0 & 0 & 0 & 0
	\end{pmatrix}
\]

$R_2 \times \frac{1}{7}$:
\[
	\begin{pmatrix}
		1 & 1 & 1           & 0           \\
		0 & 1 & \frac{4}{7} & \frac{1}{7} \\
		0 & 0 & 0           & 0
	\end{pmatrix}
\]

This system has infinitely many solutions because last row in the matrix in all zeros.
% END QUESTION 2 PART 2

\section*{Question 3}
Find the inverse of Matrix.

% BEGIN QUESTION 3 PART 1
\subsection*{(i)}
\[
	\begin{pmatrix}
		\frac{1}{2}(e^x + e^{-x}) & \frac{1}{2}(e^x - e^{-x}) \\
		\frac{1}{2}(e^x - e^{-x}) & \frac{1}{2}(e^x + e^{-x})
	\end{pmatrix}
\]

Let $A = \begin{pmatrix}
		\cosh x & \sinh x \\
		\sinh x & \cosh x
	\end{pmatrix}$ where $\cosh x = \frac{1}{2}(e^x + e^{-x})$ and $\sinh x = \frac{1}{2}(e^x - e^{-x})$

\begin{align}
	\det(A) = \cosh^2 x - \sinh^2 x = 1
\end{align}

\[
	A^{-1} = \begin{pmatrix}
		\cosh x  & -\sinh x \\
		-\sinh x & \cosh x
	\end{pmatrix} = \begin{pmatrix}
		\frac{1}{2}(e^x + e^{-x})  & -\frac{1}{2}(e^x - e^{-x}) \\
		-\frac{1}{2}(e^x - e^{-x}) & \frac{1}{2}(e^x + e^{-x})
	\end{pmatrix}
\]
% END QUESTION 3 PART 1

% BEGIN QUESTION 3 PART 2
\subsection*{(ii)}
\[
	\begin{pmatrix}
		\cos\theta  & \sin\theta \\
		-\sin\theta & \cos\theta
	\end{pmatrix}
\]

Let $A = \begin{pmatrix}
		\cos\theta  & \sin\theta \\
		-\sin\theta & \cos\theta
	\end{pmatrix}$

\begin{align}
	\det(A) = \cos^2\theta + \sin^2\theta = 1
\end{align}

\[
	A^{-1} = \begin{pmatrix}
		\cos\theta & -\sin\theta \\
		\sin\theta & \cos\theta
	\end{pmatrix}
\]
% END QUESTION 3 PART 2

% BEGIN QUESTION 3 PART 3
\subsection*{(iii)}
\[
	\begin{pmatrix}
		1 & 2 & 3 \\
		2 & 5 & 3 \\
		1 & 0 & 8
	\end{pmatrix}
\]

\[
	\begin{pmatrix}
		1 & 2 & 3 & 1 & 0 & 0 \\
		2 & 5 & 3 & 0 & 1 & 0 \\
		1 & 0 & 8 & 0 & 0 & 1
	\end{pmatrix}
\]

$R_2 - 2R_1$:
\[
	\begin{pmatrix}
		1 & 2  & 3  & 1  & 0 & 0 \\
		0 & 1  & -3 & -2 & 1 & 0 \\
		1 & 0 & 8 & 0 & 0 & 1
	\end{pmatrix}
\]

$R_3 - R_1$:
\[
	\begin{pmatrix}
		1 & 2  & 3  & 1  & 0 & 0 \\
		0 & 1  & -3 & -2 & 1 & 0 \\
		0 & -2 & 5  & -1 & 0 & 1
	\end{pmatrix}
\]

$R_3 + 2R_2$:
\[
	\begin{pmatrix}
		1 & 2 & 3  & 1  & 0 & 0 \\
		0 & 1 & -3 & -2 & 1 & 0 \\
		0 & 0 & -1 & -5 & 2 & 1
	\end{pmatrix}
\]

$R_3 \times (-1)$:
\[
	\begin{pmatrix}
		1 & 2 & 3  & 1  & 0  & 0  \\
		0 & 1 & -3 & -2 & 1  & 0  \\
		0 & 0 & 1  & 5  & -2 & -1
	\end{pmatrix}
\]

$R_2 + 3R_3$:
\[
	\begin{pmatrix}
		1 & 2 & 3 & 1 & 0  & 0  \\
		0 & 1 & 0 & 13  & -5 & -3 \\
		0 & 0 & 1  & 5  & -2 & -1
	\end{pmatrix}
\]

$R_1 - 3R_3$:
\[
	\begin{pmatrix}
		1 & 2 & 0 & -14 & 6  & 3  \\
		0 & 1 & 0 & 13  & -5 & -3 \\
		0 & 0 & 1 & 5   & -2 & -1
	\end{pmatrix}
\]

$R_1 - 2R_2$:
\[
	\begin{pmatrix}
		1 & 0 & 0 & -40 & 16 & 9  \\
		0 & 1 & 0 & 13  & -5 & -3 \\
		0 & 0 & 1 & 5   & -2 & -1
	\end{pmatrix}
\]

\[
	A^{-1} = \begin{pmatrix}
		-40 & 16 & 9  \\
		13  & -5 & -3 \\
		5   & -2 & -1
	\end{pmatrix}
\]
% END QUESTION 3 PART 3

% BEGIN QUESTION 3 PART 4
\subsection*{(iv)}
\[
	\begin{pmatrix}
		-1 & 3 & -4 \\
		2  & 4 & 1  \\
		-4 & 2 & -9
	\end{pmatrix}
\]

\[
	\begin{pmatrix}
		-1 & 3 & -4 & 1 & 0 & 0 \\
		2  & 4 & 1  & 0 & 1 & 0 \\
		-4 & 2 & -9 & 0 & 0 & 1
	\end{pmatrix}
\]

$R_1 \times (-1)$:
\[
	\begin{pmatrix}
		1 & -3 & 4  & -1 & 0 & 0 \\
		2 & 4  & 1  & 0  & 1 & 0 \\
		-4 & 2  & -9 & 0  & 0 & 1
	\end{pmatrix}
\]

$R_2 - 2R_1$:
\[
	\begin{pmatrix}
		1 & -3 & 4  & -1 & 0 & 0 \\
		0 & 10 & -7 & 2  & 1 & 0 \\
		-4 & 2  & -9 & 0  & 0 & 1
	\end{pmatrix}
\]

$R_3 + 4R_1$:
\[
	\begin{pmatrix}
		1 & -3  & 4   & -1 & 0 & 0 \\
		0 & 10  & -7  & 2  & 1 & 0 \\
		0 & -10 & 7   & -4 & 0 & 1
	\end{pmatrix}
\]

$R_3 + R_2$:
\[
	\begin{pmatrix}
		1 & -3 & 4  & -1 & 0 & 0 \\
		0 & 10 & -7 & 2  & 1 & 0 \\
		0 & 0  & 0  & -2 & 1 & 1
	\end{pmatrix}
\]

We have a row with all zeros in the left matrix so the original matrix has no inverse.
% END QUESTION 3 PART 4

% BEGIN QUESTION 3 PART 5
\subsection*{(v)}
\[
	\begin{pmatrix}
		\frac{1}{5} & \frac{1}{5}  & -\frac{2}{5} \\
		\frac{1}{5} & \frac{1}{5}  & \frac{1}{10} \\
		\frac{1}{5} & -\frac{4}{5} & \frac{1}{10}
	\end{pmatrix}
\]

Multiply by 10:
\[
	\begin{pmatrix}
		2 & 2  & -4 & 10 & 0  & 0  \\
		2 & 2  & 1  & 0  & 10 & 0  \\
		2 & -8 & 1  & 0  & 0  & 10
	\end{pmatrix}
\]

$R_1 \times \frac{1}{2}$:
\[
	\begin{pmatrix}
		1 & 1  & -2 & 5 & 0  & 0  \\
		2 & 2  & 1  & 0 & 10 & 0  \\
		2 & -8 & 1  & 0 & 0  & 10
	\end{pmatrix}
\]

$R_2 - 2R_1$:
\[
	\begin{pmatrix}
		1 & 1   & -2 & 5   & 0  & 0  \\
		0 & 0   & 5  & -10 & 10 & 0  \\
		2 & -8 & 1  & 0 & 0  & 10
	\end{pmatrix}
\]

$R_3 - 2R_1$:
\[
	\begin{pmatrix}
		1 & 1   & -2 & 5   & 0  & 0  \\
		0 & 0   & 5  & -10 & 10 & 0  \\
		0 & -10 & 5  & -10 & 0  & 10
	\end{pmatrix}
\]

$R_2 \leftrightarrow R_3$:
\[
	\begin{pmatrix}
		1 & 1   & -2 & 5   & 0  & 0  \\
		0 & -10 & 5  & -10 & 0  & 10 \\
		0 & 0   & 5  & -10 & 10 & 0
	\end{pmatrix}
\]

$R_2 \times (-\frac{1}{10})$:
\[
	\begin{pmatrix}
		1 & 1 & -2           & 5   & 0  & 0  \\
		0 & 1 & -\frac{1}{2} & 1   & 0  & -1 \\
		0 & 0 & 5            & -10 & 10 & 0
	\end{pmatrix}
\]

$R_3 \times \frac{1}{5}$:
\[
	\begin{pmatrix}
		1 & 1 & -2           & 5  & 0 & 0  \\
		0 & 1 & -\frac{1}{2} & 1  & 0 & -1 \\
		0 & 0 & 1            & -2 & 2 & 0
	\end{pmatrix}
\]

$R_2 + \frac{1}{2}R_3$:
\[
	\begin{pmatrix}
		1 & 1 & -2 & 5  & 0 & 0  \\
		0 & 1 & 0 & 0  & 1 & -1 \\
		0 & 0 & 1 & -2 & 2 & 0
	\end{pmatrix}
\]

$R_1 + 2R_3$:
\[
	\begin{pmatrix}
		1 & 1 & 0 & 1  & 4 & 0  \\
		0 & 1 & 0 & 0  & 1 & -1 \\
		0 & 0 & 1 & -2 & 2 & 0
	\end{pmatrix}
\]

$R_1 - R_2$:
\[
	\begin{pmatrix}
		1 & 0 & 0 & 1  & 3 & 1  \\
		0 & 1 & 0 & 0  & 1 & -1 \\
		0 & 0 & 1 & -2 & 2 & 0
	\end{pmatrix}
\]

\[
	A^{-1} = \begin{pmatrix}
		\frac{1}{10} & \frac{3}{10} & \frac{1}{10}  \\
		0            & \frac{1}{10} & -\frac{1}{10} \\
		-\frac{1}{5} & \frac{1}{5}  & 0
	\end{pmatrix}
\]
% END QUESTION 3 PART 5

% BEGIN QUESTION 3 PART 6
\subsection*{(vi)}
\[
	\begin{pmatrix}
		\frac{1}{5} & \frac{1}{5}  & -\frac{2}{5}  \\
		\frac{2}{5} & -\frac{3}{5} & -\frac{3}{10} \\
		\frac{1}{5} & -\frac{4}{5} & \frac{1}{10}
	\end{pmatrix}
\]

Multiply by 10 to avoid fractions:
\[
	\begin{pmatrix}
		2 & 2  & -4 & 10 & 0  & 0  \\
		4 & -6 & -3 & 0  & 10 & 0  \\
		2 & -8 & 1  & 0  & 0  & 10
	\end{pmatrix}
\]

$R_1 \times \frac{1}{2}$:
\[
	\begin{pmatrix}
		1 & 1  & -2 & 5 & 0  & 0  \\
		4 & -6 & -3 & 0 & 10 & 0  \\
		2 & -8 & 1  & 0 & 0  & 10
	\end{pmatrix}
\]

$R_2 - 4R_1$:
\[
	\begin{pmatrix}
		1 & 1   & -2 & 5   & 0  & 0  \\
		0 & -10 & 5  & -20 & 10 & 0  \\
		2 & -8  & 1  & 0   & 0  & 10
	\end{pmatrix}
\]

$R_3 - 2R_1$:
\[
	\begin{pmatrix}
		1 & 1   & -2 & 5   & 0  & 0  \\
		0 & -10 & 5  & -20 & 10 & 0  \\
		0 & -10 & 5  & -10 & 0  & 10
	\end{pmatrix}
\]

$R_3 - R_2$:
\[
	\begin{pmatrix}
		1 & 1   & -2 & 5   & 0  & 0  \\
		0 & -10 & 5  & -20 & 10 & 0  \\
		0 & 0   & 0  & 10  & -10 & 10
	\end{pmatrix}
\]

We have a row with all zeros in the left matrix so the original matrix has no inverse.
% END QUESTION 3 PART 6

\section*{Question 4}
Systems with Parameters
\[
	\begin{aligned}
		4x_1 - 7x_2 & = b_1 \\
		x_1 + 2x_2  & = b_2
	\end{aligned}
\]

\begin{itemize}
	\item[(i)] $b_1 = 0, b_2 = 1$
	\item[(ii)] $b_1 = -4, b_2 = 6$
	\item[(iii)] $b_1 = -1, b_2 = 3$
	\item[(iv)] $b_1 = -5, b_2 = 1$
\end{itemize}

% BEGIN QUESTION 4 PART 1
\subsection*{(i)} $b_1 = 0, b_2 = 1$

\[
	4x_1 - 7x_2 = 0
\]
\[
	x_1 + 2x_2 = 1
\]

$A = \begin{pmatrix}
	4 & -7 \\
	1 & 2
\end{pmatrix}, \quad b = \begin{pmatrix}
	0 \\
	1
\end{pmatrix}$

$\det(A) = 4(2) - (-7)(1) = 15$

$A^{-1} = \frac{1}{15}\begin{pmatrix}
	2 & 7 \\
	-1 & 4
\end{pmatrix}$

$x = A^{-1}b = \frac{1}{15}\begin{pmatrix}
	2 & 7 \\
	-1 & 4
\end{pmatrix}\begin{pmatrix}
	0 \\
	1
\end{pmatrix} = \frac{1}{15}\begin{pmatrix}
	7 \\
	4
\end{pmatrix}$

Therefore: $x_1 = \frac{7}{15}, x_2 = \frac{4}{15}$
% END QUESTION 4 PART 1

% BEGIN QUESTION 4 PART 2
\subsection*{(ii)} $b_1 = -4, b_2 = 6$

\[
	4x_1 - 7x_2 = -4
\]
\[
	x_1 + 2x_2 = 6
\]

$A = \begin{pmatrix}
	4 & -7 \\
	1 & 2
\end{pmatrix}, \quad b = \begin{pmatrix}
	-4 \\
	6
\end{pmatrix}$

$A^{-1} = \frac{1}{15}\begin{pmatrix}
	2 & 7 \\
	-1 & 4
\end{pmatrix}$

$x = A^{-1}b = \frac{1}{15}\begin{pmatrix}
	2 & 7 \\
	-1 & 4
\end{pmatrix}\begin{pmatrix}
	-4 \\
	6
\end{pmatrix} = \frac{1}{15}\begin{pmatrix}
	-8 + 42 \\
	4 + 24
\end{pmatrix} = \frac{1}{15}\begin{pmatrix}
	34 \\
	28
\end{pmatrix}$

Therefore: $x_1 = \frac{34}{15}, x_2 = \frac{28}{15}$
% END QUESTION 4 PART 2

% BEGIN QUESTION 4 PART 3
\subsection*{(iii)} $b_1 = -1, b_2 = 3$

\[
	4x_1 - 7x_2 = -1
\]
\[
	x_1 + 2x_2 = 3
\]

$A = \begin{pmatrix}
	4 & -7 \\
	1 & 2
\end{pmatrix}, \quad b = \begin{pmatrix}
	-1 \\
	3
\end{pmatrix}$

$A^{-1} = \frac{1}{15}\begin{pmatrix}
	2 & 7 \\
	-1 & 4
\end{pmatrix}$

$x = A^{-1}b = \frac{1}{15}\begin{pmatrix}
	2 & 7 \\
	-1 & 4
\end{pmatrix}\begin{pmatrix}
	-1 \\
	3
\end{pmatrix} = \frac{1}{15}\begin{pmatrix}
	-2 + 21 \\
	1 + 12
\end{pmatrix} = \frac{1}{15}\begin{pmatrix}
	19 \\
	13
\end{pmatrix}$

Therefore: $x_1 = \frac{19}{15}, x_2 = \frac{13}{15}$
% END QUESTION 4 PART 3

% BEGIN QUESTION 4 PART 4
\subsection*{(iv)} $b_1 = -5, b_2 = 1$

\[
	4x_1 - 7x_2 = -5
\]
\[
	x_1 + 2x_2 = 1
\]

$A = \begin{pmatrix}
	4 & -7 \\
	1 & 2
\end{pmatrix}, \quad b = \begin{pmatrix}
	-5 \\
	1
\end{pmatrix}$

$A^{-1} = \frac{1}{15}\begin{pmatrix}
	2 & 7 \\
	-1 & 4
\end{pmatrix}$

$x = A^{-1}b = \frac{1}{15}\begin{pmatrix}
	2 & 7 \\
	-1 & 4
\end{pmatrix}\begin{pmatrix}
	-5 \\
	1
\end{pmatrix} = \frac{1}{15}\begin{pmatrix}
	-10 + 7 \\
	5 + 4
\end{pmatrix} = \frac{1}{15}\begin{pmatrix}
	-3 \\
	9
\end{pmatrix}$

Therefore: $x_1 = -\frac{1}{5}, x_2 = \frac{3}{5}$
% END QUESTION 4 PART 4

\end{document}