\subsection*{(ii)}
\begin{align*}
	2x - y - 3z  & = 0 \\
	-x + 2y - 3z & = 0 \\
	x + y + 4z   & = 0
\end{align*}

\textbf{Solution using Elimination Method:}

Given system:
\begin{align}
	2x - y - 3z  & = 0 \quad (1) \\
	-x + 2y - 3z & = 0 \quad (2) \\
	x + y + 4z   & = 0 \quad (3)
\end{align}

Step 1: Eliminate $x$ from equations (1) and (2)
Multiply equation (2) by 2: $-2x + 4y - 6z = 0$
Add to equation (1): $(2x - y - 3z) + (-2x + 4y - 6z) = 0$
\begin{align}
	3y - 9z & = 0 \quad (4)
\end{align}

Step 2: Eliminate $x$ from equations (2) and (3)
Add equations (2) and (3): $(-x + 2y - 3z) + (x + y + 4z) = 0$
\begin{align}
	3y + z & = 0 \quad (5)
\end{align}

Step 3: Solve the system of equations (4) and (5)
From equation (4): $3y - 9z = 0 \Rightarrow y = 3z$
Substitute into equation (5): $3(3z) + z = 0$
\begin{align*}
	9z + z & = 0 \\
	10z    & = 0 \\
	z      & = 0
\end{align*}

Step 4: Find $y$ and $x$
Since $z = 0$ and $y = 3z$:
\begin{align*}
	y & = 3(0) = 0
\end{align*}

Substitute $y = 0$ and $z = 0$ into equation (3):
\begin{align*}
	x + 0 + 4(0) & = 0 \\
	x            & = 0
\end{align*}

Verification: Let's check our solution $(x, y, z) = (0, 0, 0)$ in all three original equations:
\begin{align*}
	\text{Equation (1):} \quad 2(0) - 0 - 3(0)  & = 0 \quad \checkmark \\
	\text{Equation (2):} \quad -0 + 2(0) - 3(0) & = 0 \quad \checkmark \\
	\text{Equation (3):} \quad 0 + 0 + 4(0)     & = 0 \quad \checkmark
\end{align*}

Therefore, the solution is $\boxed{(x, y, z) = (0, 0, 0)}$.