\subsection*{(iii)}
\begin{align*}
	v + 3w - 2x        & = 0 \\
	2u + v - 4w + 3x   & = 0 \\
	2u + 3v + 2w - x   & = 0 \\
	-4u - 3v + 5w - 4x & = 0
\end{align*}

\textbf{Solution using Row Echelon Form:}

Reordering variables as $u, v, w, x$ and setting up the augmented matrix:
\[
	\left(\begin{array}{cccc|c}
			0  & 1  & 3  & -2 & 0 \\
			2  & 1  & -4 & 3  & 0 \\
			2  & 3  & 2  & -1 & 0 \\
			-4 & -3 & 5  & -4 & 0
		\end{array}\right)
\]

Step 1: $R_1 \leftrightarrow R_2$ (get non-zero leading element)
\[
	\left(\begin{array}{cccc|c}
			2  & 1  & -4 & 3  & 0 \\
			0  & 1  & 3  & -2 & 0 \\
			2  & 3  & 2  & -1 & 0 \\
			-4 & -3 & 5  & -4 & 0
		\end{array}\right)
\]

Step 2: $R_1 \leftarrow \frac{1}{2}R_1$ (make leading coefficient 1)
\[
	\left(\begin{array}{cccc|c}
			1  & \frac{1}{2} & -2 & \frac{3}{2} & 0 \\
			0  & 1           & 3  & -2          & 0 \\
			2  & 3           & 2  & -1          & 0 \\
			-4 & -3          & 5  & -4          & 0
		\end{array}\right)
\]

Step 3: $R_3 \leftarrow R_3 - 2R_1$ and $R_4 \leftarrow R_4 + 4R_1$
\[
	\left(\begin{array}{cccc|c}
			1 & \frac{1}{2} & -2 & \frac{3}{2} & 0 \\
			0 & 1           & 3  & -2          & 0 \\
			0 & 2           & 6  & -4          & 0 \\
			0 & -1          & -3 & 2           & 0
		\end{array}\right)
\]

Step 4: $R_3 \leftarrow R_3 - 2R_2$ and $R_4 \leftarrow R_4 + R_2$
\[
	\left(\begin{array}{cccc|c}
			1 & \frac{1}{2} & -2 & \frac{3}{2} & 0 \\
			0 & 1           & 3  & -2          & 0 \\
			0 & 0           & 0  & 0           & 0 \\
			0 & 0           & 0  & 0           & 0
		\end{array}\right)
\]

The system reduces to:
\begin{align*}
	u + \frac{1}{2}v - 2w + \frac{3}{2}x & = 0 \\
	v + 3w - 2x                          & = 0
\end{align*}

\textbf{Solution using Equation Elimination:}

Given system:
\begin{align}
	v + 3w - 2x        & = 0 \quad (1) \\
	2u + v - 4w + 3x   & = 0 \quad (2) \\
	2u + 3v + 2w - x   & = 0 \quad (3) \\
	-4u - 3v + 5w - 4x & = 0 \quad (4)
\end{align}

Step 1: Eliminate $u$ from equations (2) and (3)
Subtract equation (2) from (3): $(2u + 3v + 2w - x) - (2u + v - 4w + 3x) = 0$
\begin{align}
	2v + 6w - 4x & = 0 \quad (5)
\end{align}

Step 2: Eliminate $u$ from equations (2) and (4)
Multiply equation (2) by 2: $4u + 2v - 8w + 6x = 0$
Add to equation (4): $(4u + 2v - 8w + 6x) + (-4u - 3v + 5w - 4x) = 0$
\begin{align}
	-v - 3w + 2x & = 0 \quad (6)
\end{align}

Step 3: Compare equations (1) and (6)
From equation (1): $v + 3w - 2x = 0$
From equation (6): $-v - 3w + 2x = 0$

Adding these equations: $(v + 3w - 2x) + (-v - 3w + 2x) = 0$
This gives us: $0 = 0$ (always true)

This means equations (1) and (6) are equivalent, confirming our system has infinite solutions.

\textbf{General Solution:}

From the reduced system, we can express $u$ and $v$ in terms of free variables $w$ and $x$:

From equation (1): $v = 2x - 3w$

Substituting into the first reduced equation:
$u + \frac{1}{2}(2x - 3w) - 2w + \frac{3}{2}x = 0$
$u + x - \frac{3w}{2} - 2w + \frac{3x}{2} = 0$
$u = -\frac{5x}{2} + \frac{7w}{2}$

Therefore, the general solution is:
\begin{align*}
	u & = \frac{7w - 5x}{2}               \\
	v & = 2x - 3w                         \\
	w & = w \quad \text{(free parameter)} \\
	x & = x \quad \text{(free parameter)}
\end{align*}

Or in parametric form with parameters $s = w$ and $t = x$:
\[
	\boxed{(u, v, w, x) = \left(\frac{7s - 5t}{2}, 2t - 3s, s, t\right)}
\]
where $s, t \in \mathbb{R}$ are arbitrary parameters.