\subsection*{(i)}
\begin{align*}
	2x_1 + x_2 + 3x_3 & = 0 \quad (1) \\
	x_1 + 2x_2        & = 0 \quad (2) \\
	x_2 + x_3         & = 0 \quad (3)
\end{align*}

From equation (3): $x_3 = -x_2$

Substitute into equation (1):
\begin{align*}
	2x_1 + x_2 + 3(-x_2) &= 0 \\
	2x_1 + x_2 - 3x_2 &= 0 \\
	2x_1 - 2x_2 &= 0 \\
	x_1 - x_2 &= 0 \quad (4)
\end{align*}

Now we have:
\begin{align*}
	x_1 - x_2 &= 0 \quad (4) \\
	x_1 + 2x_2 &= 0 \quad (2)
\end{align*}

Subtract equation (4) from equation (2):
\begin{align*}
	(x_1 + 2x_2) - (x_1 - x_2) &= 0 - 0 \\
	x_1 + 2x_2 - x_1 + x_2 &= 0 \\
	3x_2 &= 0 \\
	x_2 &= 0
\end{align*}

From equation (4): $x_1 = x_2 = 0$

From equation (3): $x_3 = -x_2 = 0$

Therefore: $x_1 = 0, x_2 = 0, x_3 = 0$