\subsection*{(ii)}
\begin{align*}
2x_1 + 2x_2 + 2x_3 &= 0\\
-2x_1 + 5x_2 + 2x_3 &= 1\\
8x_1 + x_2 + 4x_3 &= -1
\end{align*}

\textbf{Solution using Gaussian Elimination:}

Setting up the augmented matrix:
\[
\left(\begin{array}{ccc|c}
2 & 2 & 2 & 0\\
-2 & 5 & 2 & 1\\
8 & 1 & 4 & -1
\end{array}\right)
\]

Step 1: $R_1 \leftarrow \frac{1}{2}R_1$ (make leading coefficient 1)
\[
\left(\begin{array}{ccc|c}
1 & 1 & 1 & 0\\
-2 & 5 & 2 & 1\\
8 & 1 & 4 & -1
\end{array}\right)
\]

Step 2: $R_2 \leftarrow R_2 + 2R_1$ and $R_3 \leftarrow R_3 - 8R_1$ (eliminate below first pivot)
\[
\left(\begin{array}{ccc|c}
1 & 1 & 1 & 0\\
0 & 7 & 4 & 1\\
0 & -7 & -4 & -1
\end{array}\right)
\]

Step 3: $R_3 \leftarrow R_3 + R_2$ (eliminate below second pivot)
\[
\left(\begin{array}{ccc|c}
1 & 1 & 1 & 0\\
0 & 7 & 4 & 1\\
0 & 0 & 0 & 0
\end{array}\right)
\]

Step 4: $R_2 \leftarrow \frac{1}{7}R_2$ (make leading coefficient 1)
\[
\left(\begin{array}{ccc|c}
1 & 1 & 1 & 0\\
0 & 1 & \frac{4}{7} & \frac{1}{7}\\
0 & 0 & 0 & 0
\end{array}\right)
\]

Since we have a row of zeros, the system has infinitely many solutions. Let $x_3 = t$ be a free parameter.

From the second row: $x_2 + \frac{4}{7}x_3 = \frac{1}{7}$
\begin{align*}
x_2 + \frac{4t}{7} &= \frac{1}{7}\\
x_2 &= \frac{1}{7} - \frac{4t}{7} = \frac{1-4t}{7}
\end{align*}

From the first row: $x_1 + x_2 + x_3 = 0$
\begin{align*}
x_1 + \frac{1-4t}{7} + t &= 0\\
x_1 &= -\frac{1-4t}{7} - t = -\frac{1-4t}{7} - \frac{7t}{7}\\
x_1 &= \frac{-(1-4t) - 7t}{7} = \frac{-1+4t-7t}{7} = \frac{-1-3t}{7}
\end{align*}

Therefore, the general solution is:
\[
\boxed{(x_1, x_2, x_3) = \left(\frac{-1-3t}{7}, \frac{1-4t}{7}, t\right)}
\]
where $t \in \mathbb{R}$ is an arbitrary parameter.

\textbf{Verification with $t = 0$:}
For $t = 0$: $(x_1, x_2, x_3) = \left(-\frac{1}{7}, \frac{1}{7}, 0\right)$
\begin{align*}
\text{Equation 1:} \quad 2\left(-\frac{1}{7}\right) + 2\left(\frac{1}{7}\right) + 2(0) &= -\frac{2}{7} + \frac{2}{7} + 0 = 0 \quad \checkmark\\
\text{Equation 2:} \quad -2\left(-\frac{1}{7}\right) + 5\left(\frac{1}{7}\right) + 2(0) &= \frac{2}{7} + \frac{5}{7} + 0 = 1 \quad \checkmark\\
\text{Equation 3:} \quad 8\left(-\frac{1}{7}\right) + \frac{1}{7} + 4(0) &= -\frac{8}{7} + \frac{1}{7} + 0 = -1 \quad \checkmark
\end{align*}