\subsection*{(i)}
\[
	\begin{pmatrix}
		\frac{1}{2}(e^x + e^{-x}) & \frac{1}{2}(e^x - e^{-x}) \\
		\frac{1}{2}(e^x - e^{-x}) & \frac{1}{2}(e^x + e^{-x})
	\end{pmatrix}
\]

\textbf{Solution:}

Let $A = \begin{pmatrix}
		\frac{1}{2}(e^x + e^{-x}) & \frac{1}{2}(e^x - e^{-x}) \\
		\frac{1}{2}(e^x - e^{-x}) & \frac{1}{2}(e^x + e^{-x})
	\end{pmatrix}$

Let $\cosh x = \frac{1}{2}(e^x + e^{-x})$ and $\sinh x = \frac{1}{2}(e^x - e^{-x})$

Then $A = \begin{pmatrix}
		\cosh x & \sinh x \\
		\sinh x & \cosh x
	\end{pmatrix}$

For a $2 \times 2$ matrix $\begin{pmatrix} a & b \\ c & d \end{pmatrix}$, the inverse is $\frac{1}{ad-bc}\begin{pmatrix} d & -b \\ -c & a \end{pmatrix}$

Calculate the determinant:
\begin{align}
	\det(A) & = (\cosh x)(\cosh x) - (\sinh x)(\sinh x) \\
	        & = \cosh^2 x - \sinh^2 x                   \\
	        & = 1 \quad \text{(hyperbolic identity)}
\end{align}

Therefore:
\[
	A^{-1} = \frac{1}{1}\begin{pmatrix}
		\cosh x  & -\sinh x \\
		-\sinh x & \cosh x
	\end{pmatrix} = \begin{pmatrix}
		\cosh x  & -\sinh x \\
		-\sinh x & \cosh x
	\end{pmatrix}
\]

Substituting back:
\[
	A^{-1} = \begin{pmatrix}
		\frac{1}{2}(e^x + e^{-x})  & -\frac{1}{2}(e^x - e^{-x}) \\
		-\frac{1}{2}(e^x - e^{-x}) & \frac{1}{2}(e^x + e^{-x})
	\end{pmatrix}
\]