\subsection*{(iii)} $b_1 = -1, b_2 = 3$

\[
	4x_1 - 7x_2 = -1
\]
\[
	x_1 + 2x_2 = 3
\]

$A = \begin{pmatrix}
	4 & -7 \\
	1 & 2
\end{pmatrix}, \quad b = \begin{pmatrix}
	-1 \\
	3
\end{pmatrix}$

$A^{-1} = \frac{1}{15}\begin{pmatrix}
	2 & 7 \\
	-1 & 4
\end{pmatrix}$

$x = A^{-1}b = \frac{1}{15}\begin{pmatrix}
	2 & 7 \\
	-1 & 4
\end{pmatrix}\begin{pmatrix}
	-1 \\
	3
\end{pmatrix} = \frac{1}{15}\begin{pmatrix}
	-2 + 21 \\
	1 + 12
\end{pmatrix} = \frac{1}{15}\begin{pmatrix}
	19 \\
	13
\end{pmatrix}$

Therefore: $x_1 = \frac{19}{15}, x_2 = \frac{13}{15}$