\subsection*{(ii)} $b_1 = -4, b_2 = 6$

\[
	4x_1 - 7x_2 = -4
\]
\[
	x_1 + 2x_2 = 6
\]

$A = \begin{pmatrix}
	4 & -7 \\
	1 & 2
\end{pmatrix}, \quad b = \begin{pmatrix}
	-4 \\
	6
\end{pmatrix}$

$A^{-1} = \frac{1}{15}\begin{pmatrix}
	2 & 7 \\
	-1 & 4
\end{pmatrix}$

$x = A^{-1}b = \frac{1}{15}\begin{pmatrix}
	2 & 7 \\
	-1 & 4
\end{pmatrix}\begin{pmatrix}
	-4 \\
	6
\end{pmatrix} = \frac{1}{15}\begin{pmatrix}
	-8 + 42 \\
	4 + 24
\end{pmatrix} = \frac{1}{15}\begin{pmatrix}
	34 \\
	28
\end{pmatrix}$

Therefore: $x_1 = \frac{34}{15}, x_2 = \frac{28}{15}$