\subsection*{(iv)} $b_1 = -5, b_2 = 1$

\textbf{Solution using Gaussian Elimination and Back Substitution:}

Given system:
\begin{align}
	4x_1 - 7x_2 & = -5 \\
	x_1 + 2x_2  & = 1
\end{align}

Setting up the augmented matrix:
\[
	\left(\begin{array}{cc|c}
			4 & -7 & -5 \\
			1 & 2  & 1
		\end{array}\right)
\]

Step 1: $R_1 \leftrightarrow R_2$ (swap rows to get leading 1)
\[
	\left(\begin{array}{cc|c}
			1 & 2  & 1  \\
			4 & -7 & -5
		\end{array}\right)
\]

Step 2: $R_2 \leftarrow R_2 - 4R_1$ (eliminate below pivot)
\[
	\left(\begin{array}{cc|c}
			1 & 2   & 1  \\
			0 & -15 & -9
		\end{array}\right)
\]

Step 3: $R_2 \leftarrow -\frac{1}{15}R_2$ (make leading coefficient 1)
\[
	\left(\begin{array}{cc|c}
			1 & 2 & 1                          \\
			0 & 1 & \frac{9}{15} = \frac{3}{5}
		\end{array}\right)
\]

Step 4: $R_1 \leftarrow R_1 - 2R_2$ (eliminate above pivot)
\[
	\left(\begin{array}{cc|c}
			1 & 0 & 1 - 2 \cdot \frac{3}{5} \\
			0 & 1 & \frac{3}{5}
		\end{array}\right)
\]

Calculating $1 - 2 \cdot \frac{3}{5} = 1 - \frac{6}{5} = \frac{5}{5} - \frac{6}{5} = -\frac{1}{5}$

\[
	\left(\begin{array}{cc|c}
			1 & 0 & -\frac{1}{5} \\
			0 & 1 & \frac{3}{5}
		\end{array}\right)
\]

\textbf{Back Substitution:}

From the reduced form, we can directly read:
\begin{align*}
	x_1 & = -\frac{1}{5} \\
	x_2 & = \frac{3}{5}
\end{align*}

Therefore, the solution is $\boxed{\left(x_1, x_2\right) = \left(-\frac{1}{5}, \frac{3}{5}\right)}$.